One-line proof for all processor refinements

examples/ProcDecSC.v
@@ -88,33 +88,15 @@ Section ProcDecSC.
     kinv_red; kinv_contra.
 
   Definition decInstConfig :=
-    {| inlining := true;
+    {| inlining := ITManual;
        decomposition := DTFunctional pdec_pinst_regMap pdec_pinst_ruleMap;
        invariants := IVCons procDec_inv_ok IVNil
     |}.
 
   Lemma pdec_refines_pinst: pdec <<== pinst.
   Proof. (* SKIP_PROOF_ON
-
-    kinline_left im.
-    kdecompose_nodefs pdec_pinst_regMap pdec_pinst_ruleMap.
-
-    kinv_add procDec_inv_ok.
-    kinv_add_end.
-
-    kinvert.
-
-    - kinv_magic_with procDec_inv_old.
-    - kinv_magic_with procDec_inv_old.
-    - kinv_magic_with procDec_inv_old.
-    - kinv_magic_with procDec_inv_old.
-    - kinv_magic_with procDec_inv_old.
-    - kinv_magic_with procDec_inv_old.
-    - kinv_magic_with procDec_inv_old.
-    - kinv_magic_with procDec_inv_old.
-    - kinv_magic_with procDec_inv_old.
-
-      END_SKIP_PROOF_ON *) admit.
+    kami_ok decInstConfig procDec_inv_old idtac.
+    END_SKIP_PROOF_ON *) admit.
   Qed.
 
 End ProcDecSC.
